code/ecdsap256/Hacl.Impl.P256.Scalar.fsti
@@ -21,47 +21,49 @@ val qmod_short: x:felem -> res:felem -> Stack unit
   (ensures fun h0 _ h1 -> modifies (loc res) h0 h1 /\
     as_nat h1 res == as_nat h0 x % S.order)
 
+let qmont_R = pow2 256
+let qmont_R_inv = S.modp_inv2_prime (pow2 256) S.order
 
-noextract
-val fromDomain_: a:nat -> Tot (r:nat{r < S.order})
+let fromDomain_ (a:nat) : S.qelem = a * qmont_R_inv % S.order
+let toDomain_   (a:nat) : S.qelem = a * qmont_R % S.order
 
-noextract
-val toDomain_: a:nat -> Tot nat
+// TODO: rm if we expose the defs of fromDomain and toDomain
+val lemmaFromDomain: a:nat -> Lemma (fromDomain_ a == a * qmont_R_inv % S.order)
+val lemmaToDomain:   a:nat -> Lemma (toDomain_ a == a * qmont_R % S.order)
 
-
-val lemmaFromDomain: a:nat ->
-  Lemma ((a * S.modp_inv2_prime (pow2 256) S.order) % S.order == fromDomain_ a)
-
-val lemmaToDomain: a:nat -> Lemma ((a * pow2 256) % S.order == toDomain_ a)
-
-val lemmaFromDomainToDomain: a:nat{a < S.order} -> Lemma (toDomain_ (fromDomain_ a) == a)
-
-val lemmaToDomainFromDomain: a:nat{a < S.order} -> Lemma (fromDomain_ (toDomain_ a) == a)
+val lemmaFromDomainToDomain: a:S.qelem -> Lemma (toDomain_ (fromDomain_ a) == a)
+val lemmaToDomainFromDomain: a:S.qelem -> Lemma (fromDomain_ (toDomain_ a) == a)
 
 
-val montgomery_multiplication_ecdsa_module: a:felem -> b:felem -> result:felem -> Stack unit
+// rename with qmul
+val montgomery_multiplication_ecdsa_module: a:felem -> b:felem -> res:felem -> Stack unit
   (requires fun h ->
-    live h a /\ live h b /\ live h result /\
+    live h a /\ live h b /\ live h res /\
     eq_or_disjoint a b /\
     as_nat h a < S.order /\ as_nat h b < S.order)
-  (ensures fun h0 _ h1 -> modifies (loc result) h0 h1 /\
-    as_nat h1 result = (as_nat h0 a * as_nat h0 b * S.modp_inv2_prime (pow2 256) S.order) % S.order /\
-    as_nat h1 result = toDomain_ (fromDomain_ (as_nat h0 a) * fromDomain_ (as_nat h0 b) % S.order))
+  (ensures fun h0 _ h1 -> modifies (loc res) h0 h1 /\
+    as_nat h1 res = (as_nat h0 a * as_nat h0 b * qmont_R_inv) % S.order /\
+    as_nat h1 res = toDomain_ (fromDomain_ (as_nat h0 a) * fromDomain_ (as_nat h0 b) % S.order))
+
+// rename with qadd
+// NOTE: changed precondition `eq_or_disjoint x y`
+val felem_add: x:felem -> y:felem -> res:felem -> Stack unit
+  (requires fun h ->
+    live h x /\ live h y /\ live h res /\
+    eq_or_disjoint x y /\ eq_or_disjoint x res /\ eq_or_disjoint y res /\
+    as_nat h x < S.order /\ as_nat h y < S.order)
+  (ensures  fun h0 _ h1 -> modifies (loc res) h0 h1 /\
+    as_nat h1 res == (as_nat h0 x + as_nat h0 y) % S.order)
+
+// rename with qadd_lemma
+val lemma_felem_add: a:nat -> b:nat ->
+  Lemma ((fromDomain_ a + fromDomain_ b) % S.order = fromDomain_ (a + b))
 
 
-inline_for_extraction noextract
-val felem_add: arg1:felem -> arg2:felem -> out:felem -> Stack unit
-  (requires fun h0 ->
-    live h0 arg1 /\ live h0 arg2 /\ live h0 out /\
-    eq_or_disjoint arg1 out /\ eq_or_disjoint arg2 out /\
-    as_nat h0 arg1 < S.order /\ as_nat h0 arg2 < S.order)
-  (ensures  fun h0 _ h1 -> modifies (loc out) h0 h1 /\
-    as_nat h1 out == (as_nat h0 arg1 + as_nat h0 arg2) % S.order)
-
-val lemma_felem_add: a:nat -> b:nat -> Lemma ((fromDomain_ a + fromDomain_ b) % S.order = fromDomain_ (a + b))
-
-
-val fromDomainImpl: a:felem -> result:felem -> Stack unit
-  (requires fun h -> live h a /\ live h result /\ as_nat h a < S.order)
-  (ensures fun h0 _ h1 -> modifies (loc result) h0 h1 /\
-     as_nat h1 result < S.order /\ as_nat h1 result == fromDomain_ (as_nat h0 a))
+// rename
+val fromDomainImpl: a:felem -> res:felem -> Stack unit
+  (requires fun h ->
+    live h a /\ live h res /\ as_nat h a < S.order)
+  (ensures fun h0 _ h1 -> modifies (loc res) h0 h1 /\
+     as_nat h1 res < S.order /\
+     as_nat h1 res == fromDomain_ (as_nat h0 a))
